* now with minimization

Kleene.v
@@ -4,10 +4,17 @@ Import VectorNotations.
 
 Section to_be_moved.
 
+(** Random stuff about vectors to be placed elsewhere. *)
 Lemma hd_tl : forall {A} {n} (v:t A (S n)), v = hd v :: tl v.
 intros.
 revert n v; refine (@caseS _ _ _).
 simpl; auto.
+Qed.
+
+Lemma eq_nth_iff' {A} {n} (v1 v2:t A n) : (forall (p:Fin.t n), v1[@p] = v2[@p]) <-> v1 = v2.
+split.
+intro; apply eq_nth_iff; intros; rewrite H0; auto.
+intros; apply eq_nth_iff; auto.
 Qed.
 
 Fixpoint map_inv {A} {B} {n} (f:t (A->B) n) (x:A) : t B n :=
@@ -16,18 +23,18 @@ Fixpoint map_inv {A} {B} {n} (f:t (A->B) n) (x:A) : t B n :=
   | (f0 :: fs) => (f0 x) :: (map_inv fs x)
   end.
 
-Lemma nth_map' {A B} (f: A -> B) {n} v (p: Fin.t n): (map f v) [@p] = f (v [@p]).
+Lemma nth_map' {A B} (f: A -> B) {n} v (p: Fin.t n) : (map f v) [@p] = f (v [@p]).
 apply nth_map; auto.
 Qed.
 
-Lemma nth_map_inv {A} {B} {n} (f:t (A->B) n) v (p1 p2: Fin.t n) (eq: p1 = p2):
+Lemma nth_map_inv {A} {B} {n} (f:t (A->B) n) v (p1 p2: Fin.t n) (eq: p1 = p2) :
   (map_inv f v) [@ p1] = f[@ p2] v.
 subst p2; induction p1.
   revert n f; refine (@caseS _ _ _); now simpl.
   revert n f p1 IHp1; refine (@caseS _  _ _); now simpl.
 Qed.
 
-Lemma nth_map_inv' {A} {B} {n} (f:t (A->B) n) v (p: Fin.t n): (map_inv f v) [@p] = f[@p] v.
+Lemma nth_map_inv' {A} {B} {n} (f:t (A->B) n) v (p: Fin.t n) : (map_inv f v) [@p] = f[@p] v.
 apply nth_map_inv; auto.
 Qed.
 
@@ -51,6 +58,32 @@ Inductive PRFunction : nat -> Set :=
   | Minimization : forall {k:nat} (h:PRFunction (1+k)), PRFunction k
 .
 
+(*
+Fixpoint eval_opt {m} (f:PRFunction m) (steps:nat) (ns:t (option nat) m) : option nat :=
+  match f with
+  | Zero      => Some 0
+  | Successor => match (nth ns (Fin.of_nat_lt (Nat.lt_succ_diag_r 0))) with
+                 | Some x => Some (x + 1)
+                 | None   => None
+                 end
+  | _ => None
+  end.
+
+ -- does not work because it doesn't know Successor is PRFunction 1.
+*)
+
+(* Auxiliary function for minimization. *)
+Fixpoint find_zero_from {k} (f:t (option nat) (1+k) -> option nat) (ns:t (option nat) k) (init:nat) (steps:nat) : option nat :=
+  match steps with
+  | O   => None
+  | S m => match f ((Some init) :: ns) with
+           | None       => None
+           | Some O     => Some init
+           | Some (S _) => find_zero_from f ns (S init) m
+end end.
+
+(* We'd love a readable definition, but the dependent type of f makes it tricky to write. So... *)
+(* First we define the fixpoint construction over the option type, to cater for undefinedness. *)
 Fixpoint eval_opt {m} (f:PRFunction m) : forall (steps:nat) (ns:t (option nat) m), option nat.
 destruct f; intros.
 
@@ -82,39 +115,37 @@ destruct f; intros.
 (* Minimization *)
 + destruct steps.
   - apply None.
-  - 
-apply None.
+  - apply (find_zero_from (eval_opt _ f steps) ns 0 steps).
 Defined.
 
+(* This is the one we actually want to use. *)
 Definition eval {m} (f:PRFunction m) (steps:nat) (ns:t nat m) : option nat := eval_opt f steps (map Some ns).
+
+(* Hmmm. *)
+Lemma eval_mon : forall m (f:PRFunction m) steps ns k, eval f steps ns = (Some k) ->
+  forall s', s' > steps -> eval f s' ns = (Some k).
+unfold eval.
+assert
+  (forall (m : nat) (f : PRFunction m) (steps : nat) (ns : t (option nat) m) (k : nat),
+    eval_opt f steps ns = Some k -> forall s' : nat, s' > steps -> eval_opt f s' ns = Some k).
+2: intros; apply H with steps; auto.
+induction f; intros.
++ simpl; auto.
++ simpl; auto.
++ simpl; auto.
++ simpl; simpl in H.
+  apply IHf with steps; auto.
+  replace (map_inv (map_inv (map eval_opt f0) s') ns) with (map_inv (map_inv (map eval_opt f0) steps) ns); auto.
+  apply eq_nth_iff'; intros.
+  repeat rewrite nth_map_inv'.
+  rewrite nth_map'.
+  Abort.
+
 
 End Definitions.
 
-Section Examples.
-
-Lemma aux01 : 0 < 1.
-auto with arith.
-Qed.
-
-Lemma aux13 : 1 < 3.
-auto with arith.
-Qed.
-
-Definition PR_add := Recursion (Projection 1 0 aux01) (Composition Successor [Projection 3 1 aux13]).
-
-Eval compute in (eval PR_add 0 [2; 3]).
-Eval compute in (eval PR_add 0 [5; 7]).
-
-Definition PR_sign := Composition (Recursion Zero
-  (Composition Successor [Composition Zero [Projection 3 1 aux13]]))
-  [Projection 1 0 aux01; Projection 1 0 aux01].
-
-Eval compute in (eval PR_sign 0 [32]).
-Eval compute in (eval PR_sign 0 [0]).
-
-End Examples.
-
 Section Sanity_Checks.
+(** Since our definition of eval is very indirect, we prove that it behaves as expected. *)
 
 Lemma Zero_correct : forall n steps, eval Zero steps [n] = Some 0.
 compute; auto.
@@ -170,6 +201,29 @@ simpl (map Some (x :: t)) in H0.
 simpl; simpl in H0; rewrite H0; auto.
 Qed.
 
+Lemma Minimization_correct : forall k (h:PRFunction (1+k)) (ns:t nat k) steps n,
+  eval (Minimization h) steps ns = (Some n) ->
+  eval h steps (n::ns) = (Some 0) /\ forall m, m < n -> exists n', eval h steps (n::ns) = (Some (S n')).
+Abort.
+
+End Sanity_Checks.
+
+Section Examples.
+(** We recover the examples from the submitted journal paper. *)
+
+Lemma aux01 : 0 < 1.
+auto with arith.
+Qed.
+
+Lemma aux13 : 1 < 3.
+auto with arith.
+Qed.
+
+Definition PR_add := Recursion (Projection 1 0 aux01) (Composition Successor [Projection 3 1 aux13]).
+
+Eval compute in (eval PR_add 0 [2; 3]).
+Eval compute in (eval PR_add 0 [5; 7]).
+
 (* OMG *)
 Lemma add_correct : forall m n steps, eval PR_add steps [m; n] = Some (m + n).
 intros; induction m.
@@ -181,4 +235,24 @@ replace (m+n+1) with (S (m+n)); auto.
 rewrite (plus_comm (m+n) 1); auto with arith.
 Qed.
 
-End Sanity_Checks.
+Definition PR_sign := Composition (Recursion Zero
+  (Composition Successor [Composition Zero [Projection 3 1 aux13]]))
+  [Projection 1 0 aux01; Projection 1 0 aux01].
+
+Eval compute in (eval PR_sign 0 [32]).
+Eval compute in (eval PR_sign 0 [0]).
+
+Lemma sign_correct_0 : forall steps, eval PR_sign steps [0] = Some (0).
+intros; simpl; auto.
+Qed.
+
+Lemma sign_correct_S : forall m steps, eval PR_sign steps [S m] = Some (1).
+intros; induction m.
+simpl; auto.
+unfold PR_sign.
+revert IHm; unfold eval; simpl; intro.
+rewrite IHm; auto.
+Qed.
+
+End Examples.
+
